\documentclass[letterpaper,12pt]{article}
\input{preamble}

\chead{Coordinates and Change of Basis}

\begin{document}

Recall that if $B$ is a basis for a vector space $V$, then every vector $\vec{x} \in V$ can be written uniquely as a linear combination of the vectors of $B$. The scalars which make up this linear combination are called the \textbf{coordinates of $\vec{x}$ relative to $B$}.

\begin{definition}
Let $V$ be a vector space, $B = \set{\vec{v}_1, \dots, \vec{v}_n}$ be an ordered basis, $\vec{x} \in V$ with
\begin{equation*}
    \vec{x} = a_1 \vec{v}_1 + \dots + a_n \vec{v}_n
\end{equation*}
Then, the scalars $a_1, \dots, a_n$ are the \textbf{coordinates of $\vec{x}$ relative to the basis $B$}. The \textbf{coordinate vector} (or \textbf{coordinate matrix}) of $\vec{x}$ relative to $B$, is the column vector in $\mathbb{R}^n$ whose components are the coordinate of $\vec{x}$,
\begin{equation*}
    [\vec{x}]_B = \begin{bmatrix} a_1 \\ \vdots \\ a_n \end{bmatrix}
\end{equation*}
\end{definition}

Note that the basis is ordered, so the coordinates are ordered.

\section*{Change of Basis}

\begin{definition}
Let $B = \set{\vec{v}_1, \dots, \vec{v}_n}, B' = \set{\vec{u}_1, \dots, \vec{u}_n}$ are basis of $V$, and $\vec{x} \in V$ with coordinate vectors,
\begin{equation*}
    [\vec{x}]_B = \begin{bmatrix} a_1 \\ \vdots \\ a_n \end{bmatrix} \qquad [\vec{x}]_{B'} = \begin{bmatrix} b_1 \\ \vdots \\ b_n \end{bmatrix}
\end{equation*}
Then, the \textbf{transition matrix} from $B'$ to $B$ is the matrix $P$ such that,
\begin{equation*}
    [\vec{x}]_B = P [\vec{x}]_{B'}
\end{equation*}
\end{definition}


\begin{theorem}
If $P$ is the transition matrix from a basis $B'$ to a basis $B$ in $\mathbb{R}^n$, then $P$ is invertible and the transition matrix from $B$ to $B'$ is $P^{-1}$.
\end{theorem}



\section*{Misc Change of Coordinates}


\begin{example}
Let $R: \mathbb{R}^2 \rightarrow \mathbb{R}^2$ be a map that is reflection across the line $L$, $2x + 3y = 0$, or $L = \Span{\begin{pmatrix} 3 \\ -2 \end{pmatrix}}$.
\\ \\ We want to determine the matrix $[R]$ with respect to the standard basis $\phi = (e_1, e_2)$.
\\ \\ Formula is $[R]_{\phi}^{\phi} = [id]_{\phi}^B [R]_{B}^B [id]_B^{\phi}$
\\ \\ The change of basis matrix is $\begin{pmatrix} 3 & 2 \\ -2 & 3 \end{pmatrix}$
\\ \\ $B$ is the basis $\begin{pmatrix} 3 \\ -2 \end{pmatrix}$, $\begin{pmatrix} 2 \\ 3 \end{pmatrix}$
\\ \\ Thus, $[R] = \begin{pmatrix} 3 & 2 \\ -2 & 3 \end{pmatrix} [R]_B^B \begin{pmatrix} 3 & 2 \\ -2 & 3 \end{pmatrix}^{-1}$
\\ \\ We get
\begin{align*}
    R\begin{pmatrix} x' \\ y' \end{pmatrix} & = \begin{pmatrix} x' \\ -y' \end{pmatrix} \\
    & = \begin{pmatrix} 1 & 0 \\ 0 & -1 \end{pmatrix} \begin{pmatrix} x' \\ y' \end{pmatrix} \\
    [R]_B^B = \begin{pmatrix} 1 & 0 \\ 0 & -1 \end{pmatrix}
\end{align*}
Alternatively, $R\begin{pmatrix} 3 \\ -2 \end{pmatrix} = \begin{pmatrix} 3 \\ -2 \end{pmatrix} = 1 \begin{pmatrix} 3 \\ -2 \end{pmatrix} + 0 \begin{pmatrix} 2 \\ 3 \end{pmatrix}$
\\ \\ And, $R\begin{pmatrix} 2 \\ 3 \end{pmatrix} = \begin{pmatrix} 3 \\ -2 \end{pmatrix} = 0 \begin{pmatrix} 3 \\ -2 \end{pmatrix} -1 \begin{pmatrix} 2 \\ 3 \end{pmatrix}$
Thus,
$[R]_{\phi}^{\phi} = \begin{pmatrix} 3 & 2 \\ -2 & 3 \end{pmatrix} \begin{pmatrix} 1 & 0 \\ 0 & -1 \end{pmatrix} \begin{pmatrix} 3 & 2 \\ -2 & 3 \end{pmatrix}^{-1}$
\end{example}

\begin{example}
Let $R_{\theta}$ be rotation by $\theta$ counter-clockwise in $\mathbb{R}^2$. Rotate the coordinate system $B = (R_{\theta}e_1, R_{\theta}e_2)$
\\ \\ Change of basis matrix $[id]_{\phi}^B = (R_{\theta}e_1, R_{\theta}e_2) = R_{\theta}I_2 = R_{\theta}$
\\ \\ The change of basis matrix is equal to the rotation matrix.
\\ \\ $[v]_B = [id]_B^{\phi} [v]_{\phi}$
\\ $[v]_B = R_{\theta}^{-1} [v]_{\phi}$
\\ $\begin{pmatrix} x' \\ y' \end{pmatrix} = R_{\theta}^{-1} \begin{pmatrix} x \\ y \end{pmatrix}$
\\ The inverse of the change of basis matrix, $R_{\theta}^{-1}$, converts into new coordinates.
\end{example}

\end{document}