\documentclass[letterpaper,12pt]{article}
\input{preamble}

\chead{Transpose of a Matrix}

\begin{document}

\section*{Transpose of a Matrix}
\begin{definition}
Let $A$ be a $m \times n$ matrix. The \textbf{transpose} of $A$, $A^T$, is the matrix that results from switching the rows and columns of $A$. The $k$th row becomes the $k$th column, and vise versa. In other words,
\begin{align*}
    (A^T)_{ij} = A_{ji}
\end{align*}
\begin{itemize}
    \item As a linear map, If $A: \mathbb{F}^n \rightarrow \mathbb{F}^m$, then $A^t: \mathbb{F}^m \rightarrow \mathbb{F}^n$ is a linear map in the opposite direction.
\end{itemize}
\end{definition}

\begin{theorem}
The transpose of a transpose is equal to the original matrix.
\begin{equation*}
(A^t)^t = A
\end{equation*}
\end{theorem}
\begin{proof}
Let $A = (a_{ij})$. Then,
\begin{align*}
    (A^t)^t = ((a_{ij})^t)^t = (a_{ji})^t = (a_{ij}) = A
\end{align*}

\end{proof}

\begin{theorem} Transposition is linear. In other words, for $A, B \in M(m \times n, \mathbb{F})$, $\lambda \in \mathbb{F}$, we have
\begin{enumerate}
    \item $(A + B)^t = A^t + B^t$
    \item $(\lambda A^t) = \lambda A^t$
\end{enumerate}
\end{theorem}
\begin{proof}
\begin{enumerate}
    \item[]
    \item Let $A, B \in M(m \times n, \mathbb{F})$. Then, $(A + B)^t = (a_{ij} + b_{ij})^t = a_{ji} + b_{ji} = A^t + B^t$.
    \item Let $\lambda \in \mathbb{F}$. Then, $(\lambda A)^t = (\lambda a_{ij})^t = \lambda a_{ji} = \lambda A^t$.
\end{enumerate}
\end{proof}

\section*{Transpose of a Product}
\begin{theorem}
Let $A \in M(m \times n, \mathbb{F})$, $B \in M(n \times p, \mathbb{F})$. Then, the transpose of the product $BA$ is the reverse product of the transposes. In other words,
\begin{equation*}
    (AB)^t = B^t A^t
\end{equation*}
\begin{itemize}
    \item As linear maps, $B: \mathbb{F}^n \rightarrow \mathbb{F}^m$ and $A: \mathbb{F}^m \rightarrow \mathbb{F}^p$, so $AB: \mathbb{F}^n \rightarrow \mathbb{F}^p$.
    \\ Thus, considering the transpose (reverse order), $A^t: \mathbb{F}^p \rightarrow \mathbb{F}^m$ and $B^t: \mathbb{F}^m \rightarrow \mathbb{F}^n$, so $B^tA^t: \mathbb{F}^p \rightarrow \mathbb{F}^n$.
\end{itemize}
\end{theorem}
\begin{proof}
\begin{align*}
    (AB)^t_{ij} & = (AB)_{ji} && \text{definition of transpose} \\
    & = \sum_{k=1}^n A_{jk} B_{ki} && \text{definition of matrix multiplication} \\
    & = \sum_{k=1}^n A^t_{kj} B^t_{ik} && \text{definition of transpose} \\
    & = \sum_{k=1}^n B^t_{ik} A^t_{kj} \\
    (AB)^t_{ij} & = (B^t A^t)_{ij} && \text{definition of matrix multiplication} \\
\end{align*}
\end{proof}

\end{document}